add more examples (complete)

Examples.thy
@@ -2,7 +2,8 @@ theory Examples
   imports FOF_Base
 begin
 
-(*tautological*)
+section \<open>tautology\<close>
+
 definition f1 :: "(string, string, string) formula" where
 "f1 = Or (Not (Pred ''A'' [Var ''x''])) (Pred ''A'' [Var ''x''])"
 
@@ -15,34 +16,6 @@ definition f3 :: "(string, string, string) formula" where
 definition f4 :: "(string, string, string) formula" where
 "f4 = Exists ''x'' (Exists ''y'' 
       (Or (Equal (Var ''x'') (Var ''y'')) (Not (Equal (Var ''x'') (Var ''y'')))))"
-
-(*satisfiable*)
-definition f5 :: "(string, string, string) formula" where
-"f5 = Equiv (Pred ''A'' [Var ''x'']) (Pred ''B'' [Var ''x''])"
-
-definition f6 :: "(string, string, string) formula" where
-"f6 = undefined"
-
-definition f7 :: "(string, string, string) formula" where
-"f7 = undefined"
-
-definition f8 :: "(string, string, string) formula" where
-"f8 = undefined"
-
-(*unsatisfiable*)
-definition f9 :: "(string, string, string) formula" where
-"f9 = And (Not (Pred ''A'' [Var ''x''])) (Pred ''A'' [Var ''x''])"
-
-definition f10 :: "(string, string, string) formula" where
-"f10 = Forall ''x'' (Not (Equal (Var ''x'') (Var ''x'')))"
-
-definition f11 :: "(string, string, string) formula" where
-"f11 = And (Pred ''A'' []) (And (Pred ''B'' []) (Not (Or (Pred ''A'' []) (Pred ''B'' []))))"
-
-definition f12 :: "(string, string, string) formula" where
-"f12 = Exists ''x'' (Exists ''y'' 
-      (And (Equal (Var ''x'') (Var ''y'')) (Not (Equal (Var ''x'') (Var ''y'')))))"
-
 
 lemma f1_is_tautology:  "eval_formula f1 vI fI pI"
   unfolding f1_def
@@ -60,61 +33,96 @@ lemma f4_is_tautology:  "eval_formula f4 vI fI pI"
   unfolding f4_def
   by simp
 
-lemma f5_is_satisfiable: "\<exists>pI. eval_formula f5 vI fI pI" 
+section \<open>satisfiable\<close>
+
+definition f5 :: "(string, string, string) formula" where
+"f5 = Equiv (Pred ''A'' [Fun ''f'' [Var ''x'']]) (Pred ''B'' [Fun ''f'' [Var ''x'']])"
+
+definition f6 :: "(string, string, string) formula" where
+"f6 = Forall ''x'' (Pred ''A'' [Var ''x''])"
+
+definition f7 :: "(string, string, string) formula" where
+"f7 = And (Forall ''x'' (Exists ''y'' (Equal (Var ''x'') (Var ''y'')))) (Pred ''A'' [Var ''z''])"
+
+definition f8 :: "(string, string, string) formula" where
+"f8 = Or (And (Pred ''A'' []) (Pred ''B'' [])) (And (Pred ''A'' []) (Not (Pred ''B'' [])))"
+
+definition f9 :: "(string, string, string) formula" where
+"f9 = Imp (Pred ''B'' []) (Pred ''A'' [])"
+
+definition f10 :: "(string, string, string) formula" where
+"f10 = Not (And (Pred ''A'' []) (Pred ''B'' []))"
+
+lemma f5_is_satisfiable: "\<exists>vI fI pI. eval_formula f5 vI fI pI" 
   unfolding f5_def Equiv_def Imp_def
   by auto
 
-lemma f5_is_not_tautology: "\<exists>pI. \<not> eval_formula f5 vI fI pI"
-proof (rule exI)
+lemma f5_is_not_tautology: "\<exists>pI vI fI. \<not> eval_formula f5 vI fI pI"
+proof (rule exI) 
   let ?pI = "\<lambda> p args. (if p = ''A'' then True else False)"
-  show "\<not> eval_formula f5 vI fI ?pI"
+  show "\<exists>vI fI. \<not> eval_formula f5 vI fI ?pI"
     unfolding f5_def Equiv_def Imp_def
     by simp
 qed
 
-lemma f6_is_satisfiable: "\<exists>pI. eval_formula f6 vI fI pI" 
+lemma f6_is_satisfiable: "\<exists>vI pI. eval_formula f6 vI fI pI" 
   unfolding f6_def
-  sorry
+  by auto
 
-lemma f6_is_not_tautology: "\<exists>pI. \<not> eval_formula f6 vI fI pI"
-proof (rule exI)
-  let ?pI = "undefined"
-  show "\<not> eval_formula f6 vI fI ?pI"
-    unfolding f6_def
-    sorry
-qed
+lemma f6_is_not_tautology: "\<exists>vI pI. \<not> eval_formula f6 vI fI pI"
+  unfolding f6_def
+  by auto
 
-lemma f7_is_satisfiable: "\<exists>pI. eval_formula f7 vI fI pI" 
+lemma f7_is_satisfiable: "\<exists>vI pI. eval_formula f7 vI fI pI" 
   unfolding f7_def
-  sorry
+  by auto
 
-lemma f7_is_not_tautology: "\<exists>pI. \<not> eval_formula f7 vI fI pI"
-proof (rule exI)
-  let ?pI = "undefined"
-  show "\<not> eval_formula f7 vI fI ?pI"
-    unfolding f7_def
-    sorry
-qed
+lemma f7_is_not_tautology: "\<exists>vI pI. \<not> eval_formula f7 vI fI pI"
+  unfolding f7_def
+  by auto
 
 lemma f8_is_satisfiable: "\<exists>pI. eval_formula f8 vI fI pI" 
   unfolding f8_def
-  sorry
+  by auto
 
 lemma f8_is_not_tautology: "\<exists>pI. \<not> eval_formula f8 vI fI pI"
-proof (rule exI)
-  let ?pI = "undefined"
-  show "\<not> eval_formula f8 vI fI ?pI"
-    unfolding f8_def
-    sorry
+  unfolding f8_def
+  by auto
+
+lemma f9_is_satisfiable: "\<exists>pI. eval_formula f9 vI fI pI" 
+  unfolding f9_def Imp_def
+  by auto
+
+lemma f9_is_not_tautology: "\<exists>pI. \<not> eval_formula f9 vI fI pI"
+proof (rule exI) 
+  let ?pI = "\<lambda> p args. (if p = ''B'' then True else False)"
+  show "\<not> eval_formula f9 vI fI ?pI"
+    unfolding f9_def Imp_def
+    by simp
 qed
 
-lemma unsatisfiable_f9: "\<not> eval_formula f9 vI fI pI"
-  unfolding f9_def
-  by simp
-
-lemma unsatisfiable_f10: "\<not> eval_formula f10 vI fI pI"
+lemma f10_is_satisfiable: "\<exists>pI. eval_formula f10 vI fI pI" 
   unfolding f10_def
-  by simp
+  by auto
+
+lemma f10_is_not_tautology: "\<exists>pI. \<not> eval_formula f10 vI fI pI"
+  unfolding f10_def
+  by auto
+
+section \<open>unsatisfiable\<close>
+
+definition f11 :: "(string, string, string) formula" where
+"f11 = And (Not (Pred ''A'' [Var ''x''])) (Pred ''A'' [Var ''x''])"
+
+definition f12 :: "(string, string, string) formula" where
+"f12 = Forall ''x'' (Not (Equal (Var ''x'') (Var ''x'')))"
+
+definition f13 :: "(string, string, string) formula" where
+"f13 = And (Pred ''A'' []) (And (Pred ''B'' []) (Not (Or (Pred ''A'' []) (Pred ''B'' []))))"
+
+definition f14 :: "(string, string, string) formula" where
+"f14 = Exists ''x'' (Exists ''y'' 
+      (And (Equal (Var ''x'') (Var ''y'')) (Not (Equal (Var ''x'') (Var ''y'')))))"
 
 lemma unsatisfiable_f11: "\<not> eval_formula f11 vI fI pI"
   unfolding f11_def
@@ -122,6 +130,14 @@ lemma unsatisfiable_f11: "\<not> eval_formula f11 vI fI pI"
 
 lemma unsatisfiable_f12: "\<not> eval_formula f12 vI fI pI"
   unfolding f12_def
+  by simp
+
+lemma unsatisfiable_f13: "\<not> eval_formula f13 vI fI pI"
+  unfolding f13_def
+  by simp
+
+lemma unsatisfiable_f14: "\<not> eval_formula f14 vI fI pI"
+  unfolding f14_def
   by simp
 
 end
